tableaux v1

GPDLBisimulation/GPDL.lean
@@ -4,29 +4,345 @@ section
 variable
   {σ : Type u}
   {t : Type v}
-  {T : List t}
-  [DecidableEq t]
   [DecidableEq σ]
+  [BEq σ]
+  [BEq t]
 
-inductive Formula (σ : Type u) (T : List t)
-  | atom_prop : {p // p ∈ T} → Formula σ T
-  | top : Formula σ T
-  | neg : Formula σ T → Formula σ T
-  | and : Formula σ T → Formula σ T → Formula σ T
-  | diamond : GKAT.Exp σ T → Formula σ T → Formula σ T
+inductive Formula (σ : Type u) (t : Type v)
+  | atom_prop : t → Formula σ t
+  | top : Formula σ t
+  | neg : Formula σ t → Formula σ t
+  | and : Formula σ t → Formula σ t → Formula σ t
+  | diamond : GKAT.Exp σ t → Formula σ t → Formula σ t
+deriving BEq
 
-def Formula.bot : Formula σ T := Formula.neg Formula.top
+def Formula.bot : Formula σ t := Formula.neg Formula.top
 
-def Formula.or : Formula σ T → Formula σ T → Formula σ T
+def Formula.or : Formula σ t → Formula σ t → Formula σ t
   | φ₁, φ₂ => .neg (.and (.neg φ₁) (.neg φ₂))
 
-def Formula.impl : Formula σ T → Formula σ T → Formula σ T
+def Formula.impl : Formula σ t → Formula σ t → Formula σ t
   | φ₁, φ₂ => .neg (.and φ₁ (.neg φ₂))
 
-def formula.box : GKAT.Exp σ T → Formula σ T → Formula σ T
+def Formula.box : GKAT.Exp σ t → Formula σ t → Formula σ t
   | π, φ => .neg (.diamond π (.neg φ))
 
-structure Model (σ : Type u) (T : List t) where
+structure Model (σ : Type u) (t : Type v) where
   W : Type w
-  R : σ → W → W
-  V : {p // p ∈ T} → W → Bool
+  Ws : List W
+  R : σ → W → Option W
+  V : t → List W
+
+def bexp2formula : GKAT.BExp t → Formula σ t
+  | .one => .top
+  | .prim b => .atom_prop b
+  | .and b c => .and (bexp2formula b) (bexp2formula c)
+  | .not b => .neg (bexp2formula b)
+
+def PrefFormula (σ : Type u) (t : Type v) := List σ × Formula σ t
+
+def findContra : List (PrefFormula σ t) → Bool
+  | [] => False
+  | (s, f) :: fs =>
+    List.any fs (fun (s', f') =>
+      s == s' && (f == .neg f' || f' == .neg f)) || findContra fs
+
+def complexityB : GKAT.BExp t → Nat
+  | .and b c => (complexityB b) + (complexityB c) + 1
+  | .not b => (complexityB b) + 1
+  | _ => 1
+
+def complexityProg : GKAT.Exp σ t → Nat
+  | .do _ => 1
+  | .assert b => complexityB b + 1
+  | .seq f g => complexityProg f + complexityProg g + 1
+  | .if b f g => complexityB b + complexityProg f + complexityProg g + 1
+  | .while b f => complexityB b + complexityProg f
+
+def complexity : Formula σ t → Nat
+  | .neg f => complexity f + 1
+  | .and f1 f2 => complexity f1 + complexity f2 + 1
+  | .diamond (p) f => complexityProg p + complexity f
+  | _ => 1
+
+omit [BEq t] in
+theorem compBeqF {σ : Type u} (b : GKAT.BExp t) : complexityB b = complexity (bexp2formula b : Formula σ t) := by
+  induction b <;> simp [bexp2formula, complexityB, complexity]
+  case and b c ih1 ih2 => rw [ih1, ih2]
+  case not b ih => rw [ih]
+
+omit [BEq σ] [BEq t] in
+theorem complexityBPos (b : GKAT.BExp t) : 0 < complexityB b := by
+  induction b <;> rw [complexityB] <;> grind
+
+omit [BEq σ] [BEq t] [DecidableEq σ] in
+theorem complexityProgPos (p : GKAT.Exp σ t) : 0 < complexityProg p := by
+  induction p <;> rw [complexityProg] <;> try grind
+
+omit [BEq σ] [BEq t] [DecidableEq σ] in
+theorem complexityPos (f : Formula σ t) : 0 < complexity f := by
+  induction f <;> rw [complexity] <;> grind
+
+def complexityP : PrefFormula σ t → Nat
+  | (_, f) => complexity f
+
+def closed_tableau
+  (exp : List (PrefFormula σ t))
+  (unexp : List (PrefFormula σ t)) : Bool :=
+  if findContra (exp ++ unexp) then true else
+  match unexp with
+  | [] => false
+  | (s, f) :: fs => match f with
+    | .neg (.neg f') =>
+      have : complexityP (s, f') < complexityP (s, f'.neg.neg) := by
+        simp [complexityP, complexity]; grind
+      closed_tableau ((s, f) :: exp) ((s,f') :: fs)
+
+    | .and f1 f2 =>
+      have : complexityP (s, f1) + (complexityP (s, f2) + (List.map complexityP fs).sum) < complexityP (s, f1.and f2) + (List.map complexityP fs).sum := by
+        simp [complexityP, complexity]; grind
+      closed_tableau ((s, f) :: exp) ((s,f1) :: (s, f2) :: fs)
+
+    | .neg (.and f1 f2) =>
+      have : complexityP (s, f1.neg) < complexityP (s, (f1.and f2).neg) := by
+        simp [complexityP, complexity]; grind
+      have : complexityP (s, f2.neg) < complexityP (s, (f1.and f2).neg) := by
+        simp [complexityP, complexity]; grind
+      closed_tableau ((s, f) :: exp) ((s, .neg f1) :: fs) &&
+      closed_tableau ((s, f) :: exp) ((s, .neg f2) :: fs)
+
+    | .diamond (.do p) f' =>
+      have : complexityP (p :: s, f') < complexityP (s, Formula.diamond (GKAT.Exp.do p) f') := by
+        simp [complexityP, complexity]; exact complexityProgPos (GKAT.Exp.do p)
+      closed_tableau ((s, f) :: exp) (((p :: s), f') :: fs)
+
+    | .neg (.diamond (.do p) f') =>
+      have : complexityP (p :: s, f'.neg) < complexityP (s, (Formula.diamond (GKAT.Exp.do p) f').neg) := by
+        simp [complexityP, complexity]; exact complexityProgPos (GKAT.Exp.do p)
+      if (exp ++ unexp).any (fun (s', _) => s' == (p :: s))
+      then closed_tableau ((s, f) :: exp) (((p :: s), .neg f') :: fs)
+      else closed_tableau ((s, f) :: exp) fs
+
+    | .diamond (.assert b) f' =>
+      have : complexityP (s, bexp2formula b) + (complexityP (s, f') + (List.map complexityP fs).sum) <
+        complexityP (s, Formula.diamond (GKAT.Exp.assert b) f') + (List.map complexityP fs).sum := by
+        simp [complexityP, complexity, complexityProg]; rw [compBeqF b, Nat.add_assoc]
+        simp [Nat.add_comm (complexity (bexp2formula b)) 1]; exact lt_one_add (complexity (bexp2formula b))
+      closed_tableau ((s, f) :: exp) ((s, bexp2formula b) :: (s, f') :: fs)
+
+    | .neg (.diamond (.assert b) f') =>
+      have : complexityP (s, (bexp2formula b).neg) < complexityP (s, (Formula.diamond (GKAT.Exp.assert b) f').neg) := by
+        simp [complexityP, complexity, complexityProg]; rw [compBeqF b]
+        apply Nat.lt_add_right (complexity f'); exact lt_add_one (complexity (bexp2formula b))
+      have : complexityP (s, f'.neg) < complexityP (s, (Formula.diamond (GKAT.Exp.assert b) f').neg) := by
+        simp [complexityP, complexity]; exact complexityProgPos (GKAT.Exp.assert b)
+      closed_tableau ((s, f) :: exp) (((s, .neg (bexp2formula b))) :: fs) &&
+      closed_tableau ((s, f) :: exp) ((s, .neg f') :: fs)
+
+    | .diamond (.seq p1 p2) f' =>
+      have : complexityP (s, Formula.diamond p1 (Formula.diamond p2 f')) < complexityP (s, Formula.diamond (p1.seq p2) f') := by
+        simp [complexityP, complexity, complexityProg]; grind
+      closed_tableau ((s, f) :: exp) ((s, .diamond p1 (.diamond p2 f')) :: fs)
+
+    | .neg (.diamond (.seq p1 p2) f') =>
+      have : complexityP (s, (Formula.diamond p1 (Formula.diamond p2 f')).neg) <
+      complexityP (s, (Formula.diamond (p1.seq p2) f').neg) := by
+        simp [complexityP, complexity, complexityProg]; grind
+      closed_tableau ((s, f) :: exp) ((s, .neg (.diamond p1 (.diamond p2 f'))) :: fs)
+
+    | .diamond (.if b p1 p2) f' =>
+      have : complexityP (s, bexp2formula b) + (complexityP (s, Formula.diamond p1 f') + (List.map complexityP fs).sum) <
+        complexityP (s, Formula.diamond (GKAT.Exp.if b p1 p2) f') + (List.map complexityP fs).sum := by
+        simp [complexityP, complexity, complexityProg]; rw [compBeqF b, ←Nat.add_assoc, ←Nat.add_assoc]
+        apply Nat.add_lt_add_right; apply Nat.add_lt_add_right; rw [Nat.add_assoc, Nat.add_assoc]
+        apply Nat.add_lt_add_left; apply Nat.lt_add_of_pos_right; exact Nat.zero_lt_succ (complexityProg p2)
+      have : complexityP (s, (bexp2formula b).neg) + (complexityP (s, Formula.diamond p2 f') + (List.map complexityP fs).sum) <
+        complexityP (s, Formula.diamond (GKAT.Exp.if b p1 p2) f') + (List.map complexityP fs).sum := by
+        simp [complexityP, complexity, complexityProg]; rw [compBeqF b, ←Nat.add_assoc, ←Nat.add_assoc]
+        apply Nat.add_lt_add_right; apply Nat.add_lt_add_right; rw [Nat.add_assoc, Nat.add_assoc, Nat.add_assoc]
+        apply Nat.add_lt_add_left; rw [Nat.add_comm]; apply Nat.lt_add_of_pos_left; exact complexityProgPos p1
+      closed_tableau ((s, f) :: exp) (((s, bexp2formula b)) :: (s, .diamond p1 f') :: fs) &&
+      closed_tableau ((s, f) :: exp) (((s, .neg (bexp2formula b))) :: (s, .diamond p2 f') :: fs)
+
+    | .neg (.diamond (.if b p1 p2) f') =>
+      have : complexityP (s, bexp2formula b) + (complexityP (s, (Formula.diamond p1 f').neg) + (List.map complexityP fs).sum) <
+      complexityP (s, (Formula.diamond (GKAT.Exp.if b p1 p2) f').neg) + (List.map complexityP fs).sum := by
+        simp [complexityP, complexity, complexityProg]; rw [compBeqF b, ←Nat.add_assoc]; apply Nat.add_lt_add_right
+        rw [←Nat.add_assoc, ←Nat.add_assoc]; apply Nat.add_lt_add_right; apply Nat.add_lt_add_right
+        rw [Nat.add_assoc, Nat.add_assoc]; apply Nat.add_lt_add_left
+        apply Nat.lt_add_of_pos_right; exact Nat.zero_lt_succ (complexityProg p2)
+      have : complexityP (s, (bexp2formula b).neg) + (complexityP (s, (Formula.diamond p2 f').neg) + (List.map complexityP fs).sum) <
+      complexityP (s, (Formula.diamond (GKAT.Exp.if b p1 p2) f').neg) + (List.map complexityP fs).sum := by
+        simp [complexityP, complexity, complexityProg]; rw [compBeqF b, ←Nat.add_assoc]
+        apply Nat.add_lt_add_right; rw [←Nat.add_assoc, ←Nat.add_assoc]; apply Nat.add_lt_add_right
+        apply Nat.add_lt_add_right; rw [Nat.add_assoc, Nat.add_assoc, Nat.add_assoc]; apply Nat.add_lt_add_left
+        rw [Nat.add_comm, Nat.add_comm (complexityProg p1) (complexityProg p2 + 1)]
+        apply Nat.lt_add_of_pos_right; exact complexityProgPos p1
+      closed_tableau ((s, f) :: exp) (((s, bexp2formula b)) :: (s, .neg (.diamond p1 f')) :: fs) &&
+      closed_tableau ((s, f) :: exp) (((s, .neg (bexp2formula b))) :: (s, .neg (.diamond p2 f')) :: fs)
+
+    | f' =>
+      have : 0 < complexityP (s, f') := complexityPos f'
+      closed_tableau ((s, f) :: exp) fs
+termination_by List.sum (List.map complexityP unexp)
+
+
+partial def closed_tableau'
+  (exp : List (PrefFormula σ t))
+  (unexp : List (PrefFormula σ t)) : Bool :=
+  if findContra (exp ++ unexp) then true else
+  match unexp with
+  | (s, f) :: fs => match f with
+    | .neg (.neg f') =>
+      closed_tableau' ((s, f) :: exp) ((s,f') :: fs)
+
+    | .and f1 f2 =>
+      closed_tableau' ((s, f) :: exp) ((s,f1) :: (s, f2) :: fs)
+
+    | .neg (.and f1 f2) =>
+      closed_tableau' ((s, f) :: exp) ((s, .neg f1) :: fs) &&
+      closed_tableau' ((s, f) :: exp) ((s, .neg f2) :: fs)
+
+    | .diamond (.seq p1 p2) f' =>
+      closed_tableau' ((s, f) :: exp) ((s, .diamond p1 (.diamond p2 f')) :: fs)
+
+    | .neg (.diamond (.seq p1 p2) f') =>
+      closed_tableau' ((s, f) :: exp) ((s, .neg (.diamond p1 (.diamond p2 f'))) :: fs)
+
+    | .diamond (.assert b) f' =>
+      closed_tableau' ((s, f) :: exp) ((s, bexp2formula b) :: (s, f') :: fs)
+
+    | .neg (.diamond (.assert b) f') =>
+      closed_tableau' ((s, f) :: exp) (((s, .neg (bexp2formula b))) :: fs) &&
+      closed_tableau' ((s, f) :: exp) ((s, .neg f') :: fs)
+
+    | .diamond (.do p) f' =>
+      let x : List (PrefFormula σ t) :=
+        exp.filterMap
+          (fun pf => match pf with
+            | (s', .neg (.diamond (.do p') f'')) =>
+              if (s' == s) && (p' == p)
+              then some ((p :: s), .neg f'')
+              else none
+            | _ => none)
+      closed_tableau' ((s, f) :: exp) (((p :: s), f') :: (x ++ fs))
+
+    --!!!!!!!!!!!!!!!!!!!!!!!!!!!!!!
+    -- (p :: s) já presente no ramo
+    | .neg (.diamond (.do p) f') =>
+      if (exp ++ unexp).any (fun (s', _) => s' == (p :: s))
+      then closed_tableau' ((s, f) :: exp) (((p :: s), .neg f') :: fs)
+      else closed_tableau' ((s, f) :: exp) fs
+    --!!!!!!!!!!!!!!!!!!!!!!!!!!!!!!
+
+    | .diamond (.if b p1 p2) f' =>
+      closed_tableau' ((s, f) :: exp) (((s, bexp2formula b)) :: (s, .diamond p1 f') :: fs) &&
+      closed_tableau' ((s, f) :: exp) (((s, .neg (bexp2formula b))) :: (s, .diamond p2 f') :: fs)
+
+    | .neg (.diamond (.if b p1 p2) f') =>
+      closed_tableau' ((s, f) :: exp) (((s, bexp2formula b)) :: (s, .neg (.diamond p1 f')) :: fs) &&
+      closed_tableau' ((s, f) :: exp) (((s, .neg (bexp2formula b))) :: (s, .neg (.diamond p2 f')) :: fs)
+
+
+    | f' =>
+      closed_tableau' ((s, f) :: exp) fs
+
+  -- expandir boxes que faltem
+  | [] => false
+
+partial def closed_tableau''
+  (exp : List (PrefFormula σ t))
+  (unexp : List (PrefFormula σ t)) : Option (Model σ t) :=
+  if findContra (exp ++ unexp) then none else
+  match unexp with
+  | (s, f) :: fs => match f with
+    | .neg (.neg f') =>
+      closed_tableau'' ((s, f) :: exp) ((s,f') :: fs)
+
+    | .and f1 f2 =>
+      closed_tableau'' ((s, f) :: exp) ((s,f1) :: (s, f2) :: fs)
+
+    | .neg (.and f1 f2) =>
+      match closed_tableau'' ((s, f) :: exp) ((s, .neg f1) :: fs) with
+      | some M => some M
+      | none => closed_tableau'' ((s, f) :: exp) ((s, .neg f2) :: fs)
+
+    | .diamond (.seq p1 p2) f' =>
+      closed_tableau'' ((s, f) :: exp) ((s, .diamond p1 (.diamond p2 f')) :: fs)
+
+    | .neg (.diamond (.seq p1 p2) f') =>
+      closed_tableau'' ((s, f) :: exp) ((s, .neg (.diamond p1 (.diamond p2 f'))) :: fs)
+
+    | .diamond (.assert b) f' =>
+      closed_tableau'' ((s, f) :: exp) ((s, bexp2formula b) :: (s, f') :: fs)
+
+    | .neg (.diamond (.assert b) f') =>
+      match closed_tableau'' ((s, f) :: exp) (((s, .neg (bexp2formula b))) :: fs) with
+      | some M => some M
+      | none => closed_tableau'' ((s, f) :: exp) ((s, .neg f') :: fs)
+
+    | .diamond (.do p) f' =>
+      let x : List (PrefFormula σ t) :=
+        exp.filterMap
+          (fun pf => match pf with
+            | (s', .neg (.diamond (.do p') f'')) =>
+              if (s' == s) && (p' == p)
+              then some ((p :: s), .neg f'')
+              else none
+            | _ => none)
+      closed_tableau'' ((s, f) :: exp) (((p :: s), f') :: (x ++ fs))
+
+    --!!!!!!!!!!!!!!!!!!!!!!!!!!!!!!
+    -- (p :: s) já presente no ramo
+    | .neg (.diamond (.do p) f') =>
+      if (exp ++ unexp).any (fun (s', _) => s' == (p :: s))
+      then closed_tableau'' ((s, f) :: exp) (((p :: s), .neg f') :: fs)
+      else closed_tableau'' ((s, f) :: exp) fs
+    --!!!!!!!!!!!!!!!!!!!!!!!!!!!!!!
+
+    | .diamond (.if b p1 p2) f' =>
+      match closed_tableau'' ((s, f) :: exp) (((s, bexp2formula b)) :: (s, .diamond p1 f') :: fs)with
+      | some M => some M
+      | none => closed_tableau'' ((s, f) :: exp) (((s, .neg (bexp2formula b))) :: (s, .diamond p2 f') :: fs)
+
+    | .neg (.diamond (.if b p1 p2) f') =>
+      match closed_tableau'' ((s, f) :: exp) (((s, bexp2formula b)) :: (s, .neg (.diamond p1 f')) :: fs) with
+      | some M => some M
+      | none => closed_tableau'' ((s, f) :: exp) (((s, .neg (bexp2formula b))) :: (s, .neg (.diamond p2 f')) :: fs)
+
+
+    | f' =>
+      closed_tableau'' ((s, f) :: exp) fs
+  | [] =>
+    some {
+      W := List σ
+      Ws := (exp.map (fun (s, _) => s)).dedup
+      R :=
+        fun p s =>
+          if (exp.any (fun (s', _) => s' == (p :: s)))
+          then some (p :: s)
+          else none
+      V := fun b =>
+        (exp.filterMap
+          (fun (s, f) =>
+            if f == .atom_prop b
+            then some s
+            else none))
+    }
+
+
+def f1 : Formula Char Char :=
+  .impl
+    (.and
+      (.diamond (.if (.prim 'b') (.do 'f') (.do 'g')) (.atom_prop 'p'))
+      (.atom_prop 'b'))
+    (.diamond (.do 'f') (.atom_prop 'p'))
+
+def f2 : Formula Char Char :=
+  .impl
+    (.box (.do 'p') (.atom_prop 'f'))
+    (.diamond (.do 'p') (.atom_prop 'f'))
+
+
+
+#eval closed_tableau' [] [([], (.neg f2))]
